%% LyX 2.0.3 created this file.  For more info, see http://www.lyx.org/.
%% Do not edit unless you really know what you are doing.
\documentclass[12pt,oneside,english]{amsart}
\usepackage[T1]{fontenc}
\usepackage[latin9]{inputenc}
\usepackage{geometry}
\geometry{verbose,tmargin=2.5cm,bmargin=2.5cm,lmargin=2.5cm,rmargin=2.5cm}
\usepackage{amsthm}
\usepackage{amssymb}

\makeatletter
%%%%%%%%%%%%%%%%%%%%%%%%%%%%%% Textclass specific LaTeX commands.
\numberwithin{equation}{section}
\numberwithin{figure}{section}

\makeatother

\usepackage{babel}
\begin{document}
Abelson and Sussman \emph{Structure and Interpretation of Computer
Programs 2nd Edition. }Exercise 2.5.


\section*{Solution}

We show that $f:\mathbb{Z}\times\mathbb{Z}\rightarrow\mathbb{Z}$
defined by $f\left(a,b\right)=2^{a}3^{b}$, is 1-1.

Suppose that $f\left(a,b\right)=f\left(c,d\right)$. Then $2^{a}3^{b}=2^{c}3^{d}$.
Assume, for the sake of obtaining a contradiction, that $a\neq c$.
Then without loss of generality we may suppose that $a>c$. This implies
that $2^{a-c}3^{b}=3^{d}$ is even, since $a-c>0$. This is our contradiction.
Hence $a=c$. It follows immediately that $b=d$. Hence $f$ is 1-1.
\end{document}
